systems/Log.v
@@ -1,0 +1,73 @@
+Require Import Verdi.Verdi.
+
+Require Import Cheerios.Cheerios.
+
+Set Implicit Arguments.
+
+Section Log.
+  Context {orig_base_params : BaseParams}.
+  Context {orig_multi_params : MultiParams orig_base_params}.
+  Context {orig_failure_params : FailureParams orig_multi_params}.
+  Context {data_serializer : Serializer data}.
+
+  Definition log_net_handlers dst src m st : (input + msg) * list output * data * list (name * msg)  :=
+    let '(out, data, ps) := net_handlers dst src m st in
+    (inr m , out, data, ps).
+
+  Definition log_input_handlers h inp st : (input + msg) * list output * data * list (name * msg) :=
+    let '(out, data, ps) := input_handlers h inp st in
+    (inl inp, out, data, ps).
+
+  Fixpoint apply_log h (d : data) (entries : list (input + (name * msg))) : data :=
+    match entries with
+    | [] => d
+    | e :: entries =>
+      apply_log h
+                (match e with
+                 | inl inp => match log_input_handlers h inp d with
+                              | (_, _, d, _) => d
+                              end
+                 | inr (src, m) => match log_net_handlers h src m d with
+                                   | (_, _, d, _) => d
+                                   end
+                 end) 
+                entries
+    end.
+  
+  Instance log_base_params : BaseParams :=
+    {
+      data := data ;
+      input := input ;
+      output := output
+    }.
+
+  Definition init_log h :=
+    (0, init_handlers h, [] : list (input + msg)).
+  
+  Instance log_multi_params : LogMultiParams log_base_params :=
+    {
+      l_name := name;
+      l_name_eq_dec := name_eq_dec;
+      l_msg := msg;
+      l_msg_eq_dec := msg_eq_dec;
+      l_nodes := nodes;
+      l_all_names_nodes := all_names_nodes;
+      l_no_dup_nodes := no_dup_nodes;
+      l_init_handlers := init_handlers;
+      l_init_log := init_log;
+      l_net_handlers := log_net_handlers;
+      l_input_handlers := log_input_handlers
+    }.
+  
+  Instance log_failure_params : LogFailureParams log_multi_params :=
+    {
+      l_reboot := fun l =>
+                    match l with
+                    | (_, d, _) => @reboot _ _ orig_failure_params d
+                    end
+    }.  
+End Log.
+
+Hint Extern 5 (@BaseParams) => apply log_base_params : typeclass_instances.
+Hint Extern 5 (@DiskMultiParams _) => apply log_multi_params : typeclass_instances.
+Hint Extern 5 (@DiskFailureParams _ _) => apply log_failure_params : typeclass_instances.
